theories/L4_deBruijn/L3_to_L3_eta.v
@@ -1,0 +1,456 @@
+(** Naive conversion to a deBruijn-only expression language for a core calculus including
+    mutually recursive functions, data constructors, and pattern matching.
+ *)
+
+Require Import Coq.Arith.Arith Coq.NArith.BinNat Coq.Strings.String Coq.Lists.List
+        Coq.omega.Omega Coq.Program.Program Coq.micromega.Psatz.
+Require Export Common.Common.  (* shared namespace *)
+Open Scope N_scope.
+Opaque N.add.
+Opaque N.sub.
+Require Import L3.compile.
+Module L3t := L3.compile.
+Require Import L4.expression.
+
+(** Tactics *)
+Ltac forward H :=
+  match type of H with
+  | ?T -> _ => let H' := fresh in cut T;[intros H'; specialize (H H') | ]
+  end.
+
+Import L3t.
+
+Section TermTranslation.
+    
+  Fixpoint strip_lam (k : nat) (e : exp) : list name * exp :=
+    match k, e with
+    | 0%nat, _ => ([], e)
+    | S n, Lam_e na e => let '(names, e) := strip_lam n e in
+                       (na :: names, e)
+    | S n, _ => ([],e)
+    end.
+
+  (* Section fixes. *)
+  (*   Variable trans : N -> L3t.Term -> exp. *)
+  (*   Definition trans_args (k : N) (t : L3t.Terms) : exps := *)
+  (*     map_terms (trans k) t. *)
+  (*   Fixpoint trans_brs ind k n l := *)
+  (*     match l with *)
+  (*     | L3t.dnil => brnil_e *)
+  (*     | L3t.dcons na t nargs ts => *)
+  (*       let '(names, t') := strip_lam nargs (trans k t) in *)
+  (*       brcons_e (ind,n) (N.of_nat nargs, names) t' *)
+  (*                (trans_brs ind k (n + 1)%N ts) *)
+  (*     end. *)
+  (*   Fixpoint trans_fixes k l := *)
+  (*     match l with *)
+  (*     | L3t.dnil => eflnil *)
+  (*     | L3t.dcons na t _ l' => *)
+  (*       eflcons na (trans k t) (trans_fixes k l') *)
+  (*     end. *)
+
+  (* End fixes. *)
+
+  (* Move Γ |- body : τ1 -> .. -> τn -> τ to 
+     Γ, x1 : τ1, .., xn : τn |- body x1 .. xn : τ
+   *)
+  
+
+  Fixpoint is_n_lambda n t :=
+    match n with
+    | 0%nat => true
+    | S n => match t with
+            | TLambda _ t => is_n_lambda n t
+            | _ => false
+            end
+    end.
+
+  Fixpoint eta_expand_aux (n : nat) (t : Term) (k : Terms) : Term :=
+    match n with
+    | 0%nat => mkApp t (treverse k)
+    (* | S n, TLambda na t => *)
+    (*   (* Γ |- λ t : τ1 -> τ2 .. τn -> τ to  *)
+    (*      Γ, τ1 |- t : τ2 .. τn -> τ *)
+    (*    *)  *)
+    (*   TLambda na (eta_expand_aux n t k) *)
+    | S n' =>
+      TLambda nAnon (eta_expand_aux n' (lift 0 t) (tcons (TRel n') k))
+    end.
+
+  Definition eta_expand n t :=
+    if is_n_lambda n t then t
+    else eta_expand_aux n t tnil.
+      
+  Eval compute in is_n_lambda 1 (TLambda (nNamed "x") (TRel 0)).
+  Eval compute in eta_expand 1 (TLambda (nNamed "x") (TRel 0)).
+  
+  Eval compute in eta_expand 2 (TLambda (nNamed "x") (TRel 0)).
+  Eval compute in eta_expand 2 (TLambda (nNamed "x") (TRel 1)).
+    
+  Eval compute in eta_expand 3 (TRel 0).
+  Eval compute in eta_expand 1 (TLambda (nNamed "x") (TRel 0)).
+  Eval compute in eta_expand 2 (TLambda (nNamed "x") (TRel 1)).
+  
+  Fixpoint trans (k : nat) (t : Term) : Term :=
+    match t with
+    | TAx => TAx
+    | TWrong => TWrong
+    | TProof => TProof
+    | TRel n => TRel n
+    | TLambda n t => TLambda n (trans (1+k) t)
+    | TLetIn n t u => TLetIn n (trans k t) (trans (1+k) u)
+    | TApp t u => TApp (trans k t) (trans k u)
+    | TConst s => TConst s
+    | TConstruct ind c args =>      
+      TConstruct ind c (trans_terms k args)
+    | TCase ind t brs =>
+      TCase ind (trans k t) (trans_brs ind k brs)
+    | TFix d n =>
+      let len := L3t.dlength d in
+      let defs' := trans_fixes (len + k) d in
+      TFix defs' n
+    end
+
+  with trans_terms (k : nat) (ts : Terms) : Terms :=
+    match ts with
+    | tnil => tnil
+    | tcons t ts => tcons (trans k t) (trans_terms k ts)
+    end
+  with trans_brs (i : inductive) (k : nat) (brs : Defs) : Defs :=
+    match brs with
+    | dnil => dnil
+    | dcons na t n brs =>
+      let transt := trans k t in
+      let etat := eta_expand n transt in
+      dcons na etat n (trans_brs i k brs)
+    end
+  with trans_fixes (k : nat) (d : Defs) : Defs :=
+    match d with
+    | dnil => dnil
+    | dcons na t n ds => dcons na (trans k t) n (trans_fixes k ds)
+    end.
+
+  
+End TermTranslation.
+
+Require Import L3.term L3.program L3.compile L3.wcbvEval.
+
+Fixpoint transEC (ec:envClass Term) : envClass Term :=
+  match ec with
+    | ecTrm t => ecTrm (trans 0 t)
+    | ecTyp _ n itp => ecTyp _ n itp
+  end.
+
+Fixpoint transEnv (p:environ Term) : environ Term :=
+  match p with
+    | nil => nil
+    | cons (nm, ec) q => cons (nm, transEC ec) (transEnv q)
+  end.
+
+Lemma Lookup_trans_env e nm t : LookupDfn nm e t -> LookupDfn nm (transEnv e) (trans 0 t).
+Proof.
+  red. intros H. red in H.
+  dependent induction H. simpl. constructor.
+  constructor; auto.
+Qed.
+
+Lemma wcbvEval_pres_Crct e t t' :
+  crctTerm e 0 t -> WcbvEval e t t' -> crctTerm e 0 t'.
+Admitted.
+
+Inductive match_annot : list Cnstr -> Defs -> Prop :=
+| match_annot_nil : match_annot [] dnil
+| match_annot_cons na t args c cnstrs ds :
+    c.(CnstrArity) = args ->
+    match_annot cnstrs ds ->
+    match_annot (c :: cnstrs) (dcons na t args ds).
+         
+Definition crctAnn (e : environ Term) ann brs :=
+  let 'mkInd nm tndx := ann in
+  exists pack ityp,
+    LookupTyp nm e 0 pack /\
+    getInd pack tndx = Ret ityp /\
+    match_annot ityp.(itypCnstrs) brs.
+
+Lemma Crct_invrt_Case e n ann mch brs :
+  crctTerm e n (TCase ann mch brs) ->
+  crctTerm e n mch /\ crctDs e n brs /\
+  crctAnn e ann brs /\
+  (forall i t, dnth i brs = Some t -> crctTerm e n (dbody _ t)).
+Admitted.
+
+Lemma Crct_construct {e : environ Term} {i n args} : crctEnv e ->
+  crctTerm e 0 (TConstruct i n args) ->
+  cnstrArity e i n = Ret (0%nat, tlength args).
+Proof. intros. inv H. Admitted.
+
+Lemma dnthBody_trans n t i brs :
+  dnth n brs = Some t -> exists t',
+    dnth n (trans_brs i 0 brs) = Some t' /\
+    t'.(dbody _) = eta_expand (t.(rarg _)) (trans 0 t.(dbody _)).
+Proof.
+  revert n t i; induction brs; intros *.
+  simpl; intros. discriminate.
+  
+  simpl. unfold dnthBody. destruct n1. simpl.
+  intros [= <-].
+  eexists; split; eauto.
+  simpl.
+  
+  intros. now eapply IHbrs.
+Qed.
+      
+Arguments raise : simpl never.
+Arguments String.append : simpl never.
+
+Lemma match_annot_n {cnstrs brs n c t} :
+  match_annot cnstrs brs ->
+  exnNth cnstrs n = Ret c ->
+  dnth n brs = Some t -> CnstrArity c = t.(rarg _).
+Proof.
+  intros H; revert n c t; induction H; intros; simpl; auto.
+  - discriminate.
+  - destruct n. injection H1; intros ->. injection H2; intros <-.
+    simpl; auto.
+
+    simpl in H1, H2.
+    now specialize (IHmatch_annot _ _ _ H1 H2).
+Qed.
+
+Lemma WcbvEval_mkApp_einv {e f a s} : WcbvEval e (mkApp f a) s -> exists s', WcbvEval e f s'.
+Proof.
+  revert f; induction a; simpl; intros.
+  - now exists s.
+  - specialize (IHa (TApp f t) H).
+    destruct IHa.
+    inv H0.
+    * now exists TProof.
+    * now exists (TLambda nm bod).
+    * exists (TFix dts m). auto.
+    * now exists efn. 
+Qed.
+
+Lemma WcbvEval_is_n_lam e n t t' : is_n_lambda n t = true -> WcbvEval e t t' -> is_n_lambda n t' = true.
+Proof.
+  induction n; simpl; intros Hlam; auto.
+  
+  destruct t; try discriminate.
+  intros. inv H.
+  auto.
+Qed.
+
+Lemma WcbvEval_mkApp_inner e f f' s' a s :
+  let n := tlength a in
+  is_n_lambda n s' = true ->
+  WcbvEval e f s' ->
+  WcbvEval e f' s' ->
+  WcbvEval e (mkApp f a) s -> WcbvEval e (mkApp f' a) s.
+Proof.
+  revert f f' s' s; induction a; intros *; intros Hlam evf evf' evapp; simpl in *.
+  - now rewrite <- (WcbvEval_single_valued evf evapp).
+  - subst n; simpl in *.
+    destruct s'; try discriminate.
+    destruct (WcbvEval_mkApp_einv evapp) as [s'' evs''].
+    
+    assert(WcbvEval e (TApp f' t) s'').
+    { inv evs''.
+      pose proof (WcbvEval_single_valued evf H2). discriminate.
+      injection (WcbvEval_single_valued evf H1). intros -> ->.
+      econstructor; eauto.
+      pose proof (WcbvEval_single_valued evf H1). discriminate.
+      pose proof (WcbvEval_single_valued evf H1). subst efn. elim H2. red.
+      do 2 eexists ; reflexivity. }
+    eapply (IHa (TApp f t) (TApp f' t) s'' s ); auto.
+    
+    inv evs''.
+    pose proof (WcbvEval_single_valued evf H3). discriminate.
+    injection (WcbvEval_single_valued evf H2). intros -> ->.
+    eapply WcbvEval_is_n_lam. 2:apply H5. admit.
+    pose proof (WcbvEval_single_valued evf H2). discriminate.
+    pose proof (WcbvEval_single_valued evf H2). subst efn. elim H3.
+    do 2 eexists; reflexivity.
+Admitted.
+
+Lemma eval_app_terms e f args s :
+  WcbvEval e (mkApp f args) s ->
+  WcbvEval e (mkApp (eta_expand (tlength args) f) args) s.
+Proof.
+  revert e f s; induction args; intros.
+  simpl; trivial.
+
+  simpl.
+  unfold eta_expand.
+  destruct is_n_lambda. auto.
+
+  simpl.
+  Lemma WcbvEval_mkApp e f f' a s :
+    WcbvEval e f f' -> WcbvEval e (mkApp f' a) s ->
+    WcbvEval e (mkApp f a) s.
+  Proof.
+    intros evff' evf'a.
+    dependent induction evf'a.
+  Admitted.
+
+  eapply WcbvEval_mkApp.
+  eapply wAppLam. constructor. admit.
+  simpl in H. unfold whBetaStep.
+Admitted.
+    
+  
+  
+
+(* Lemma eval_app_terms e f args s : *)
+(*   WcbvEval e (mkApp f args) s -> *)
+(*   WcbvEval e (mkApp (eta_expand (tlength args) f) args) s. *)
+(* Proof. *)
+(*   revert e f s; induction args; intros. *)
+(*   simpl; trivial. *)
+  
+(*   simpl in *. specialize (IHargs _ _ _ H). unfold eta_expand. *)
+(*   case_eq (is_n_lambda (S (tlength args)) f). auto. *)
+(*   intros. *)
+
+  
+  
+(*   eapply WcbvEval_mkApp_inner. 2:apply IHargs. *)
+  
+(*   simpl. *)
+(* Admitted. *)
+
+Lemma whCase_step e i n args brs cs s :
+  crctEnv e -> crctDs e 0 brs -> crctAnn e i brs ->
+  cnstrArity e i n = Ret (0%nat, tlength args) ->
+  whCaseStep n args brs = Some cs -> WcbvEval e cs s ->
+  WcbvEval (transEnv e) (trans 0 cs) (trans 0 s) ->
+  exists cs',
+    whCaseStep n (trans_terms 0 args) (trans_brs i 0 brs) =
+    Some cs' /\ WcbvEval (transEnv e) cs' (trans 0 s).
+Proof.
+  intros crcte crctds crctann crctar Hcase Hev IHev.
+  unfold whCaseStep in Hcase.
+  revert Hcase; case_eq (dnthBody n brs). intros t Hdn [= <-].
+  unfold whCaseStep.
+  
+  unfold dnthBody in Hdn. case_eq (dnth n brs). intros. rewrite H in Hdn.
+  destruct (dnthBody_trans _ _ i _ H) as [cs' [Hnth Heq]].
+  unfold dnthBody. rewrite Hnth. destruct cs'. simpl in *.
+  eexists; split; eauto.
+  
+  subst dbody.
+  destruct d. simpl in *.
+  assert(tlength args = rarg0).
+  { unfold crctAnn in *. destruct i as [nm ndx].
+    destruct crctann as [pack [ityp [Hlook [Hind Hann]]]].
+    unfold cnstrArity in crctar. red in Hlook. destruct Hlook as [Hlook none].
+    apply Lookup_lookup in Hlook. unfold lookupTyp in *. rewrite Hlook in crctar.
+    destruct pack; try discriminate. rewrite Hind in crctar.
+    unfold getCnstr in crctar. case_eq (exnNth (itypCnstrs ityp) n).
+    intros. rewrite H0 in crctar. discriminate.
+    intros; rewrite H0 in crctar.
+    injection crctar. intros.
+    assert (me:=match_annot_n Hann H0 H). simpl in me. congruence. }
+  subst rarg0. injection Hdn ; intros <-.
+  clear Hnth H .
+
+  clear crctar Hdn.
+  revert dbody s Hev IHev.
+  induction args. simpl.
+  unfold eta_expand. simpl. trivial.
+
+  simpl; intros dbody s Hev IHev.
+  specialize (IHargs _ _ Hev IHev).
+  simpl in IHargs.
+    
+Admitted.
+  
+Theorem translate_correct_subst (e : environ Term) (t t' : Term) :
+  crctEnv e -> crctTerm e 0 t ->
+  WcbvEval e t t' -> 
+  WcbvEval (transEnv e) (trans 0 t) (trans 0 t').
+Proof.
+  assert ((forall t t' : Term,
+  WcbvEval e t t' -> 
+  crctEnv e -> crctTerm e 0 t ->
+  WcbvEval (transEnv e) (trans 0 t) (trans 0 t')) /\
+          (forall t t' : Terms,
+   WcbvEvals e t t' ->
+   crctTerms e 0 t ->
+   WcbvEvals (transEnv e) (trans_terms 0 t) (trans_terms 0 t'))).
+  clear; apply WcbvEvalEvals_ind; simpl; auto.
+
+  - intros fn arg evprf IHev crcte crctt.
+    apply Crct_invrt_App in crctt.
+    constructor. intuition eauto.
+
+  - intros i r args args' evargs evtras crcte crctc.
+    destruct i as [ipkg inum]. 
+    apply Crct_invrt_Construct in crctc.
+    intuition.
+
+  - intros nm t s Ht evalt IHt crcte crctt.
+    econstructor; [ | eapply IHt]; eauto.
+    apply Lookup_trans_env; auto.
+    eapply Crct_LookupDfn_Crct; eauto.
+
+  - intros * evfn IHfn evat IHa1 eva1' IHa1' crcte crctc.
+    apply Crct_invrt_App in crctc as [crctfn crcta1].
+    econstructor; eauto.
+
+    assert(trans 0 (whBetaStep bod a1') = whBetaStep (trans 1 bod) (trans 0 a1')).
+    admit.
+    rewrite <- H. apply IHa1'; auto.
+    eapply whBetaStep_pres_Crct.
+    apply wcbvEval_pres_Crct in evfn; auto.
+    now apply Crct_invrt_Lam in evfn.
+    apply wcbvEval_pres_Crct in evat; auto.
+
+  - intros * evdfn IHdfn evbod IHbod crcte crctt.
+    apply Crct_invrt_LetIn in crctt as [crctdn crctbod].
+    econstructor; eauto.
+    forward IHbod; auto. forward IHbod.
+    admit.
+    admit.
+
+  - intros * evfix IHfix Hfix evapp IHapp crcte crcta.
+    apply Crct_invrt_App in crcta as [crctfn crctarg].
+    eapply wAppFix with (fs := trans 0 fs). forward IHfix; auto.
+    admit.
+    apply IHapp; auto.
+    admit.
+
+  - intros * wfn IHfn notlam notfix nproof evarg IHarg crcte crcta.
+    apply Crct_invrt_App in crcta as [crctfn crctarg].
+    constructor; auto.
+    admit. admit. admit.
+
+  - intros * evmch IHmch Hcase evcs IHcs crcte crctc.
+    apply Crct_invrt_Case in crctc as [crctmch crctbrs].
+    econstructor. eauto.
+    
+Admitted.    
+    
+(** start-to-L4 translations **)
+Definition myprogram_Program : program -> Program Term :=
+  L3t.program_Program.
+(*************
+  do pgm0 <- malecha_L1.program_Program pgm (Ret nil);
+    let e' := stripEvalCommute.stripEnv (program.env pgm0) in
+    match L3U.stripEnv e' with
+    | Ret senv => 
+      match L3U.strip e' (stripEvalCommute.strip (program.main pgm0)) with
+      | Ret smain => Ret {| main := smain; L3.program.env := senv |}
+      | Exc s => Exc ("Error in stripping: " ++ s)
+      end
+    | Exc s => Exc ("Error while stripping environ L3.compile.Termment: " ++ s)
+    end.
+ *************)
+
+Definition translate_program (e : environ L3.compile.Term) (t : L3t.Term) : L3t.Term :=
+  trans 0 t.
+
+Definition Program_Program (pgm : Program L3t.Term) : Program L3t.Term :=
+  let 'mkPgm main env := pgm in
+  {| main := trans 0 main; env := transEnv env |}.
+
+Definition program_L3_eta (pgm:program) : Program L3t.Term :=
+  Program_Program (myprogram_Program pgm).
